Hs/Metatheory/Uniqueness.lean
@@ -1,1 +1,155 @@
-import Hs.CompileJ
+import Hs.Algorithm
+import Hs.HsJudgment
+
+------------------------------------
+-- Sorting Judgments
+------------------------------------
+
+theorem kinding_uniqueness :
+  Γ ⊢κ τ : k ->
+  Γ ⊢κ τ : k' ->
+  k = k' :=
+ by
+intro j1 j2
+induction τ generalizing Γ k k'
+case _ => cases j1; cases j2; rfl
+all_goals (cases j1)
+case _ ih1 ih2 kl1 kl2 =>
+  cases j2; rfl;
+
+@[simp]
+abbrev SortJudgmentUniquenessType : (v : HsVariant) -> Ctx HsTerm -> HsJudgmentArgs v -> Prop
+| .kind => λ Γ => λ (t, τ) =>
+   (j1 : Γ ⊢κ t : τ) -> (j2 : Γ ⊢κ t : τ) -> j1 = j2
+| _ => λ _ => λ _ => true
+
+theorem kinds_have_unique_judgments_lemma :
+  (∀ Γ (h1 h2 : ⊢s Γ), h1 = h2) ->
+  HsJudgment v Γ idx -> SortJudgmentUniquenessType v Γ idx
+  := by
+intro h j;
+induction j <;> simp at *;
+case _ Γ _ _ =>
+  intro j1 j2;
+  cases j1; case _ j1 =>
+  cases j2; case _ j2 =>
+  have h' := @h Γ j1 j2;
+  cases h'; simp
+case _ Γ _ _ _ _ ih1 ih2 =>
+  intro j1 j2;
+  cases j1; cases j2;
+  case _ ja1 jb1 ja2 jb2 =>
+  have h1 := @ih1 ja1 ja2;
+  have h2 := @ih2 jb1 jb2;
+  cases h1; cases h2; simp;
+
+theorem kinds_have_unique_judgments :
+  (∀ Γ (h1 h2 : ⊢s Γ), h1 = h2) ->
+  (j1 : Γ ⊢κ t : τ) ->
+  (j2 : Γ ⊢κ t : τ) ->
+  j1 = j2 := by
+intro h j1 j2;
+apply kinds_have_unique_judgments_lemma h j2 j1 j2;
+
+theorem kinds_compiling_uniqueness :
+  (∀ Γ (h1 h2 : ⊢s Γ), h1 = h2) ->
+  (j1 : Γ ⊢κ t : τ) ->
+  (j2 : Γ ⊢κ t : τ) ->
+  compile_kind Γ t τ j1 = .some t1 ->
+  compile_kind Γ t τ j2 = .some t2 ->
+  t1 = t2 := by
+intro h j1 j2 c1 c2
+have lem := kinds_have_unique_judgments h j1 j2; cases lem;
+rw[c1] at c2; injection c2
+
+------------------------------------
+-- Judgments For Types
+------------------------------------
+
+theorem types_have_unique_kinds :
+  Γ ⊢τ t : k ->
+  Γ ⊢τ t : k' ->
+  k = k' := by
+intro j1 j2;
+induction t generalizing Γ k k';
+all_goals (cases j1)
+case _ =>
+  cases j2
+  case _ h2 _ _ h1 =>
+  rw [<-h1] at h2; injection h2;
+all_goals(cases j2)
+case _ ih1 ih2 A j1 j2 A' j1' j2' =>
+  have u := @ih2 Γ A A' j1 j1'; subst u;
+  have u := @ih1 Γ (A `-k> k) (A `-k> k') j2 j2';
+  simp at u; apply u;
+case _ => rfl
+case _ => rfl
+case _ => rfl
+
+@[simp]
+abbrev KindingJudgmentsUniquessType : (v : HsVariant) -> Ctx HsTerm -> HsJudgmentArgs v -> Prop
+| .type => λ Γ => λ (t, τ) =>
+   (j1 : Γ ⊢τ t : τ) -> (j2 : Γ ⊢τ t : τ) -> j1 = j2
+| _ => λ _ => λ _ => true
+
+theorem types_have_unique_judgments_lemma :
+  (∀ Γ (h1 h2 : ⊢s Γ), h1 = h2) ->
+  HsJudgment v Γ idx -> KindingJudgmentsUniquessType v Γ idx := by
+intro h j;
+induction j <;> simp at *;
+case _ Γ _ _ ja jb ih1 ih2 =>
+  intro j1 j2;
+  cases j1; cases j2; simp at *;
+  case _ ja1 jb1 ja2 jb2 =>
+  have lem := kinds_have_unique_judgments h ja1 ja2; cases lem;
+  have lem := ih1 jb1 jb2; cases lem; simp
+case _ Γ _ _ ja jb ih1 ih2 =>
+  intro j1 j2;
+  cases j1; cases j2; simp at *;
+  case _ ja1 jb1 ja2 jb2 =>
+  have lem := types_have_unique_kinds ja1 ja2; cases lem;
+  have lem := types_have_unique_kinds ja ja1; cases lem;
+  have lem := ih1 ja1 ja2; cases lem
+  have lem := ih2 jb1 jb2; cases lem; simp
+case _ Γ _ _ ja _ jb ih1 ih2 =>
+  intro j1 j2;
+  cases j1; cases j2; simp at *;
+  case _ ja1 _ jb1 ja2 _ jb2 =>
+  have lem := types_have_unique_kinds ja1 ja2; cases lem;
+  have lem := types_have_unique_kinds ja ja1; cases lem;
+  have lem := ih1 ja1 ja2; cases lem
+  have lem := ih2 jb1 jb2; cases lem; simp
+case _ Γ _ _ _ _ jf ja ih1 ih2  =>
+  intro j1 j2;
+  cases j1; cases j2;
+  simp at *;
+  case _ ja1 jf1 _ ja2 jf2 =>
+  have lem := types_have_unique_kinds ja1 ja2; cases lem; simp at *;
+  have lem := types_have_unique_kinds ja ja1; cases lem;
+  have lem := ih1 jf1 jf2; cases lem
+  have lem := ih2 ja1 ja2; cases lem; simp
+case _ Γ _ _ _ _ _ _ =>
+  intro j1 j2;
+  cases j1; cases j2;
+  simp at *;
+  case _ wf1 _ _ wf2 _ _ => apply @h Γ wf1 wf2;
+
+theorem types_have_unique_judgments :
+  (∀ Γ (h1 h2 : ⊢s Γ), h1 = h2) ->
+  (j1 : Γ ⊢τ t : k) ->
+  (j2 : Γ ⊢τ t : k) ->
+  j1 = j2 := by
+intro h j1 j2;
+apply types_have_unique_judgments_lemma h j2 j1 j2;
+
+theorem compile_type_uniqueness :
+  (∀ Γ (h1 h2 : ⊢s Γ), h1 = h2) ->
+  (j1 : Γ ⊢τ τ : k) ->
+  (j2 : Γ ⊢τ τ : k) ->
+  compile_type Γ τ k j1 = .some t1 ->
+  compile_type Γ τ k j2 = .some t2 ->
+  t1 = t2
+  := by
+intro h j1 j2 c1 c2;
+have lem := types_have_unique_judgments h j1 j2; cases lem;
+rw[c1] at c2; injection c2;
