Hs/Metatheory/Preservation2.lean
@@ -1,25 +1,31 @@
 import Hs.Algorithm
+import Hs.Metatheory.Uniqueness
 
+-- Says how the shape of the core context changes with Hs Ctx
 inductive CompileCtx : Ctx HsTerm -> Ctx Term -> Prop where
 | nil : CompileCtx [] []
 | empty :
   ⊢s Γ ->
+  ⊢ Γ' ->
   CompileCtx Γ Γ' ->
   CompileCtx (.empty :: Γ) (.empty :: Γ')
 | kind :
   ⊢s Γ ->
+  ⊢ Γ' ->
   CompileCtx Γ Γ' ->
   (j1 : Γ ⊢κ A : `□) ->
   compile_kind Γ A `□ j1 = .some A' ->
   CompileCtx (.kind A :: Γ) (.kind A' :: Γ')
 | type :
   ⊢s Γ ->
+  ⊢ Γ' ->
   CompileCtx Γ Γ' ->
   (j1 : Γ ⊢τ A : `★) ->
   compile_type Γ A `★ j1 = .some A' ->
   CompileCtx (.type A :: Γ) (.type A' :: Γ')
 | term :
   ⊢s Γ ->
+  ⊢ Γ' ->
   CompileCtx Γ Γ' ->
   (j1 : Γ ⊢τ A : `★)  ->
   (j2 : Γ ⊢t t : τ) ->
@@ -27,50 +33,8 @@ inductive CompileCtx : Ctx HsTerm -> Ctx Term -> Prop where
   compile_term Γ t τ j2 = .some t' ->
   CompileCtx (.term A t :: Γ) (.term A' t' :: Γ')
 
-theorem compile_ctx_type :
-  CompileCtx Γ Γ' ->
-  (Γ d@ x).get_type = .some τ ->
-  (j : Γ ⊢τ `#x : τ) ->
-  compile_type Γ `#x τ j = .some τ' ->
-  (Γ' @ x).get_type = .some τ' :=
-by
-intro cc gt j c;
-unfold compile_type at c; cases j; cases c;
-case _ wf test gt =>
- clear gt;
- induction cc;
- case _ => cases test
- case _ =>
-   induction x generalizing Γ Γ';
-   case _ => cases gt;
-   case _ ih1 ih2 =>
-   sorry
- case _ => sorry
- case _ => sorry
- case _ => sorry
-
-
-theorem compile_preserves_term_indices :
-  CompileCtx Γ Γ' ->
-  (j1 : Γ ⊢t `#x : T) ->
-  compile_type Γ T k j = .some T' ->
-  (Γ' d@ x).get_type = .some T' := by
-sorry
-
-theorem kinding_uniqueness :
-  Γ ⊢κ τ : k ->
-  Γ ⊢κ τ : k' ->
-  k = k' :=
- by
-intro j1 j2
-induction τ generalizing Γ k k'
-case _ => cases j1; cases j2; rfl
-all_goals (cases j1)
-case _ ih1 ih2 kl1 kl2 =>
-  cases j2; rfl;
-
 theorem compile_preserves_kinds :
-  CompileCtx Γ Γ' ->
+  ⊢ Γ' ->
   (j : Γ ⊢κ t : τ) ->
   compile_kind Γ t τ j = .some t' ->
   Γ' ⊢ t' : .kind := by
@@ -79,9 +43,9 @@ theorem compile_preserves_kinds :
  all_goals try (cases e)
  case _ =>
    unfold compile_kind at c; cases c;
-   case _ wf => sorry
-     -- apply Judgment.ax;
-     -- apply compile_ctx_wf wf cc
+   case _ =>
+     apply Judgment.ax;
+     assumption;
  case _ j1 j2 ih1 ih2 =>
    unfold compile_kind at c; simp at c;
    rw[Option.bind_eq_some] at c;
@@ -91,53 +55,29 @@ theorem compile_preserves_kinds :
    cases c2; case _ w2 c2 =>
    cases c2; case _ c2 c3 =>
    cases c3;
-   have ih1' := @ih1 w1 cc c1;
-   have ih2' := @ih2 w2 cc c2;
+   have ih1' := ih1 c1;
+   have ih2' := ih2 c2;
    apply Judgment.allk;
    apply ih1';
    apply ih2'
 
-
-def typing_js_gives_kinding_js :
-  Γ ⊢τ t : k ->
-  Γ ⊢κ k : `□ := by
-intro j; sorry
-
-
-theorem typing_uniqueness :
-  Γ ⊢τ t : k ->
-  Γ ⊢τ t : k' ->
-  k = k' := by
-intro j1 j2;
-induction t generalizing Γ k k';
-all_goals (cases j1)
-case _ =>
-  cases j2
-  case _ h2 _ _ h1 =>
-  rw [<-h1] at h2; injection h2;
-all_goals(cases j2)
-case _ ih1 ih2 A j1 j2 A' j1' j2' =>
-  have u := @ih2 Γ A A' j1 j1'; subst u;
-  have u := @ih1 Γ (A `-k> k) (A `-k> k') j2 j2';
-  simp at u; apply u;
-case _ => rfl
-case _ => rfl
-case _ => rfl
-
 theorem compile_preserves_types :
   CompileCtx Γ Γ' ->
+  ⊢ Γ' ->
   (j2 : Γ ⊢κ k : `□) ->
   compile_kind Γ k `□ j2 = .some k' ->
   (j1 : Γ ⊢τ τ : k) ->
   compile_type Γ τ k j1 = .some τ' ->
   Γ' ⊢ τ' : k' := by
-intro cc j1 c1 j2 c2;
+intro cc wf j1 c1 j2 c2;
 induction Γ, τ, k, j2 using compile_type.induct generalizing Γ' τ' k'
 all_goals (unfold compile_type at c2; simp at c2)
 case _ Γ x wf test gt =>
-     cases c2; sorry
-  -- cases c2;
-  -- apply Judgment.var;
+     cases c2;
+     apply Judgment.var;
+     assumption;
+     have lem1 := compile_preserves_kinds wf j1 c1;
+     sorry
   -- apply compile_ctx_wf; assumption; assumption;
   -- have lem1 := HsJudgment.varTy wf test gt
   -- have lem := compile_preserves_type_indices cc lem1 c1; symm at lem;
@@ -150,6 +90,8 @@ case _ h1 h2 ih1 ih2 =>
   cases c3; case _ w2 c3 =>
   cases c3; case _ c3 e =>
   cases e;
+  have ih1' := @ih1 Γ'
+  have ih2' := @ih2 Γ'
   apply Judgment.appk;
   case _ => sorry;
   case _ => sorry;
@@ -164,9 +106,10 @@ case _ h1 h2 ih1 =>
   cases e; unfold compile_kind at c1; cases j1;
   simp at c1; cases c1;
   apply Judgment.allt;
-  apply compile_preserves_kinds cc h1 c2;
-  apply @ih1 (.kind w1 :: Γ') ★ w2 _ _ _ c3
-  case _ => apply CompileCtx.kind; assumption; assumption; assumption
+  apply compile_preserves_kinds wf h1 c2;
+  apply @ih1 (.kind w1 :: Γ') ★ w2 _ _ _ _ c3
+  case _ => apply sorry
+  case _ => apply sorry
   case _ => apply HsJudgment.ax; apply HsJudgment.wfkind; assumption; assumption
   case _ => unfold compile_kind; rfl
 
@@ -178,17 +121,18 @@ case _ j1 _ j2 ih1 ih2 =>
   cases c3; case _ w2 c3 =>
   cases c3; case _ c3 e =>
   cases e;
-  have lem1 := compile_preserves_kinds cc j1 c1;
+  have lem1 := compile_preserves_kinds wf j1 c1;
   unfold compile_kind at c1; simp at c1;
   cases j1; simp at c1; cases c1;
   apply Judgment.arrow;
-  apply @ih1 Γ' ★ w1 cc _ _;
-  case _ => apply c2;
+  apply @ih1 Γ' ★ w1 cc wf _ _ _;
   case _ => apply HsJudgment.ax; assumption
-  case _ => unfold compile_kind; rfl
+  case _ => sorry
+  case _ => sorry
 
-  apply @ih2 (.empty::Γ') ★ w2 _ _ _ c3
-  case _ => apply CompileCtx.empty; assumption; assumption
+  apply @ih2 (.empty::Γ') ★ w2 _ _ _ _ c3;
+  case _ => sorry
+  case _ => apply Judgment.wfempty; assumption;
   case _ => apply HsJudgment.ax; apply HsJudgment.wfempty; assumption
   case _ => unfold compile_kind; rfl
 
@@ -200,27 +144,29 @@ case _ j1 _ j2 ih1 ih2 =>
   cases c3; case _ w2 c3 =>
   cases c3; case _ c3 e =>
   cases e;
-  have lem1 := compile_preserves_kinds cc j1 c1;
+  have lem1 := compile_preserves_kinds wf j1 c1;
   unfold compile_kind at c1; simp at c1;
   cases j1; simp at c1; cases c1;
   case _ tl1 tl2 _ =>
   apply Judgment.arrow;
-  apply @ih1 Γ' ★ w1 cc _ _ c2;
+  apply @ih1 Γ' ★ w1 cc wf _ _ c2;
   case _ => apply HsJudgment.ax; assumption
   case _ => unfold compile_kind; rfl
-  apply @ih2 (.empty::Γ') ★ w2 _ _ _ c3
-  case _ => apply CompileCtx.empty; assumption; assumption
+  apply @ih2 (.empty::Γ') ★ w2 _ _ _ _ c3
+  case _ => sorry
+  case _ => sorry -- apply CompileCtx.empty; assumption; assumption
   case _ => apply HsJudgment.ax; apply HsJudgment.wfempty; assumption
   case _ => unfold compile_kind; rfl
 
 theorem compile_preserves_typing :
-  CompileCtx Γ Γ' ->
+  (∀ Γ (h1 h2 : ⊢s Γ), h1 = h2) ->
+  ⊢ Γ' ->
   (j1 : Γ ⊢τ τ : k) ->
   compile_type Γ τ k j1 = .some τ' ->
   (j2 : Γ ⊢t t : τ) ->
   compile_term Γ t τ j2 = .some t' ->
   Γ' ⊢ t' : τ' := by
-intro cc j1 c1 j2 c2;
+intro h cc j1 c1 j2 c2;
 induction Γ, t, τ, j2 using compile_term.induct generalizing Γ' t' τ' k
 all_goals (unfold compile_term at c2; simp at c2)
 case _ wf test gt => sorry
@@ -238,7 +184,7 @@ case _ j1' j2 j3 ih1 =>
  cases c3; case _ t' c3 =>
  cases c3; case _ c3 e =>
  cases e;
- have uniq := typing_uniqueness j1 j3; subst uniq;
+ have uniq := types_have_unique_kinds j1 j3; subst uniq;
  unfold compile_type at c1; cases j1; simp at c1;
  rw[Option.bind_eq_some] at c1;
  cases c1; case _ x1 c1' =>
@@ -268,17 +214,46 @@ case _ => sorry
 
 
 theorem compile_ctx_wf :
+  ⊢s Γ ->
+  (c : HsCtx Γ) ->
+  compile_ctx c = .some Γ' ->
+  ⊢ Γ' :=
+by
+intro h1 h2; sorry
+-- induction h2;
+-- case _ => apply Judgment.wfnil
+-- case _ ih1 =>
+--   case _ h1 =>
+--   apply Judgment.wfempty; assumption;
+-- case _ h1 j1 cc ih =>
+--  apply Judgment.wfkind;
+--  sorry
+--  sorry
+-- case _ => sorry
+-- case _ => sorry
+theorem compile_ctx_type : ∀ Γ Γ',
+  ⊢ Γ' ->
   CompileCtx Γ Γ' ->
-  ⊢ Γ' := by
-intro h2;
-induction h2;
-case _ => apply Judgment.wfnil
+  (Γ d@ x).get_type = .some τ ->
+  (j : Γ ⊢τ `#x : τ) ->
+  compile_type Γ `#x τ j = .some τ' ->
+  (Γ' @ x).get_type = .some τ' :=
+by
+intro Γ Γ' wf cc gt j c;
+induction cc <;> simp at *;
+case _ => cases gt
 case _ ih1 =>
-  case _ h1 =>
-  apply Judgment.wfempty; assumption;
-case _ h1 j1 cc ih =>
- apply Judgment.wfkind;
- sorry
- sorry
+  induction x;
+  case _ => simp at *; cases j; case _ j => cases j;
+  case _ ih2 => simp; sorry
 case _ => sorry
 case _ => sorry
+case _ => sorry
+-- unfold compile_type at c; cases j; cases c;
+
+theorem compile_preserves_term_indices :
+  ⊢ Γ' ->
+  (j1 : Γ ⊢t `#x : T) ->
+  compile_type Γ T k j = .some T' ->
+  (Γ' d@ x).get_type = .some T' := by
+sorry
